add test for OrigBlockTiling1D
+ create block_tiled1d matmul combinator types for GPU and host
+ add optional checks on the output of gemm kernels

test/Test_Kuiper_GEMM_SHMem__F32_GEMM.cu
@@ -3,9 +3,9 @@
 #define stem         Kuiper_GEMM_SHMem_g_gemm_
 #define et           float
 #define et_lbl       f32
+#define PRIet        "f"
 #define GEMM_ALPHA   0.7
 #define GEMM_BETA    0.3
-// #define PRIet        "f"
-#define TOLERANCE    CRAP
+#define TOLERANCE    0.001f
 
 #include "tiled_gemm_driver.c.inc"
